```agda
{-# OPTIONS --without-K --exact-split #-}

open import UF-FunExt
open import SpartanMLTT

module TernaryBoehmRealsPrelude (fe : FunExt) where

open import Two-Properties hiding (zero-is-not-one)
open import NaturalsOrder
open import NaturalsAddition renaming (_+_ to _+ℕ_)
open import IntegersB
open import IntegersOrder
open import IntegersAddition renaming (_+_ to _+ℤ_)
open import IntegersNegation renaming (-_  to  −ℤ_)
open import UF-Subsingletons
open import NaturalsOrder
open import DecidableAndDetachable

succ-lc : (x y : ℕ) → succ x ≡ succ y → x ≡ y
succ-lc x x refl = refl

ℕ-is-discrete : (x y : ℕ) → decidable (x ≡ y)
ℕ-is-discrete zero zero = inl refl
ℕ-is-discrete zero (succ y) = inr (λ ())
ℕ-is-discrete (succ x) zero = inr (λ ())
ℕ-is-discrete (succ x) (succ y)
 = Cases (ℕ-is-discrete x y)
     (inl ∘ ap succ)
     (inr ∘ λ f g → f (succ-lc x y g))

pos-lc : (x y : ℕ) → pos x ≡ pos y → x ≡ y
pos-lc x x refl = refl

negsucc-lc : (x y : ℕ) → negsucc x ≡ negsucc y → x ≡ y
negsucc-lc x x refl = refl

ℤ-is-discrete : (x y : ℤ) → decidable (x ≡ y)
ℤ-is-discrete (pos     x) (pos     y)
 = Cases (ℕ-is-discrete x y)
     (inl ∘ ap pos)
     (inr ∘ (λ f g → f (pos-lc x y g)))
ℤ-is-discrete (negsucc x) (negsucc y)
 = Cases (ℕ-is-discrete x y)
     (inl ∘ ap negsucc)
     (inr ∘ (λ f g → f (negsucc-lc x y g)))
ℤ-is-discrete (pos     _) (negsucc _) = inr (λ ())
ℤ-is-discrete (negsucc _) (pos     _) = inr (λ ())

_≤ℤ_≤ℤ_ : ℤ → ℤ → ℤ → 𝓤₀ ̇ 
x ≤ℤ y ≤ℤ z = (x ≤ℤ y) × (y ≤ℤ z)

≤ℤ²-is-prop : {l u : ℤ} (x : ℤ) → is-prop (l ≤ℤ x ≤ℤ u)
≤ℤ²-is-prop {l} {u} x = ×-is-prop (ℤ≤-is-prop l x) (ℤ≤-is-prop x u)

data 𝟛 : 𝓤₀ ̇ where
  −1 O +1 : 𝟛

_/2 : ℕ → ℕ
0 /2 = 0
1 /2 = 0
succ (succ n) /2 = succ (n /2)

sign : ℤ → (ℕ → ℤ)
sign (pos     _) = pos
sign (negsucc _) = negsucc

num : ℤ → ℕ
num  (pos     n) = n
num  (negsucc n) = n

odd even : ℤ → 𝓤₀ ̇
odd (pos                   0) = 𝟘
odd (pos                   1) = 𝟙
odd (pos (succ (succ x)))     = odd (pos x)
odd (negsucc               0) = 𝟙
odd (negsucc               1) = 𝟘
odd (negsucc (succ (succ x))) = odd (negsucc x)
even x = ¬ odd x

even-or-odd? : (x : ℤ) → even x + odd x
even-or-odd? (pos                   0) = inl (λ x → x)
even-or-odd? (pos                   1) = inr ⋆
even-or-odd? (pos (succ (succ x)))     = even-or-odd? (pos x)
even-or-odd? (negsucc               0) = inr ⋆
even-or-odd? (negsucc               1) = inl (λ x → x)
even-or-odd? (negsucc (succ (succ x))) = even-or-odd? (negsucc x)

odd-is-prop : (x : ℤ) → is-prop (odd x)
odd-is-prop (pos                   0) = 𝟘-is-prop
odd-is-prop (pos                   1) = 𝟙-is-prop
odd-is-prop (pos (succ (succ x)))     = odd-is-prop (pos x)
odd-is-prop (negsucc               0) = 𝟙-is-prop
odd-is-prop (negsucc               1) = 𝟘-is-prop
odd-is-prop (negsucc (succ (succ x))) = odd-is-prop (negsucc x)

succ-odd-is-even : (x : ℤ) → odd x → even (succℤ x)
succ-odd-is-even (pos                          1) o = id
succ-odd-is-even (pos            (succ (succ x))) o = succ-odd-is-even (pos x) o
succ-odd-is-even (negsucc                      0) o = id
succ-odd-is-even (negsucc (succ (succ (succ x)))) o = succ-odd-is-even (negsucc (succ x)) o

succ-even-is-odd : (x : ℤ) → even x → odd (succℤ x)
succ-even-is-odd (pos                          0) e = ⋆
succ-even-is-odd (pos                          1) e = e ⋆
succ-even-is-odd (pos            (succ (succ x))) e = succ-even-is-odd (pos x) e
succ-even-is-odd (negsucc                      0) e = e ⋆
succ-even-is-odd (negsucc                      1) e = ⋆
succ-even-is-odd (negsucc                      2) e = e ⋆
succ-even-is-odd (negsucc (succ (succ (succ x)))) e = succ-even-is-odd (negsucc (succ x)) e

even-is-prop : (x : ℤ) → is-prop (even x)
even-is-prop x p q = dfunext (fe _ _) (λ i → 𝟘-elim (p i))

even-or-odd-is-prop : (x : ℤ) → is-prop (even x + odd x)
even-or-odd-is-prop x = +-is-prop (even-is-prop x) (odd-is-prop x) id

_−ℤ_ : ℤ → ℤ → ℤ
x −ℤ y = x +ℤ (−ℤ y)

ℤ[_,_] : ℤ → ℤ → 𝓤₀ ̇
ℤ[ l , u ] = Σ z ꞉ ℤ , (l ≤ℤ z ≤ℤ u)

ℤ[_,_]-succ : (l u : ℤ) → ℤ[ l , u ] → ℤ[ l , succℤ u ]
ℤ[ l , u ]-succ (z , l≤z , z≤u) = z , l≤z , ℤ≤-trans z u (succℤ u) z≤u (1 , refl) 

≤ℤ-antisym : ∀ x y → x ≤ℤ y ≤ℤ x → x ≡ y
≤ℤ-antisym x y (x≤y , y≤x) with ℤ≤-split x y x≤y | ℤ≤-split y x y≤x
... | inl (n , γ) | inl (m , δ)
 = 𝟘-elim (ℤ-equal-not-less-than x (ℤ<-trans x y x (n , γ) (m , δ)))
... | inl  _  | inr y≡x = y≡x ⁻¹
... | inr x≡y | _       = x≡y

≤ℤ-back : ∀ x y → x <ℤ y → x ≤ℤ predℤ y
≤ℤ-back x .(succℤ x +ℤ pos n) (n , refl)
 = ℤ≤-trans x (x +pos n) (predℤ (succℤ x +pos n))
     (n , refl)
     (transport ((x +pos n) ≤ℤ_)
       (predsuccℤ (x +pos n) ⁻¹
       ∙ ap predℤ (ℤ-left-succ x (pos n) ⁻¹))
       (ℤ≤-refl (x +pos n)))
